Add first version of translation function

TransVal/sexp.v
@@ -1,11 +1,8 @@
 
-Require Import AllInRel List Map Env DecSolve.
-Require Import IL Annotation AutoIndTac Bisim Exp MoreExp Filter Exp Coherence Fresh.
-Require Import NPeano.
+Require Import List NPeano Decidable.
+Require Import IL.
 
 Set Implicit Arguments.
-
-Local Hint Resolve incl_empty minus_incl incl_right incl_left.
 
 (**
 First define bits to be a binary type with the two constructors O and I.
@@ -23,23 +20,25 @@ Definition bitvec := list bit.
 Definition senv:Type := var -> option bitvec.
 
 (**
-Define SMT expressions on bitvectors. For the moment I only add +,-_2,*,/,-_1constants and variables
+Define SMT expressions on bitvectors. For the moment I only add +,-_2,*,/constants and variables
 **)
 Inductive sexp :=
 |plus: sexp -> sexp -> sexp
 |sub: sexp -> sexp -> sexp
 |mult: sexp -> sexp -> sexp
 |div: sexp -> sexp -> sexp
-|neg: sexp -> sexp
+|sneg: sexp->sexp
 |const: bitvec -> sexp
 |svar: var -> sexp.
 
+(** Define a function to map a single bit to a natural number **)
 Definition bitToNat (b1:bit) :nat :=
 match b1 with
 |I => 1
 |O => 0
 end.
 
+(** For every bit there exists a number *)
 Lemma exists_number_bit:
 forall b:bit, exists n:nat, bitToNat b = n.
 
@@ -49,12 +48,14 @@ intros. destruct b.
 - exists 1. reflexivity.
 Qed.
 
+(** Now define the natural number for bitvectors **)
 Fixpoint bitvecToNat (b:list bit) :nat :=
 match b with
 |nil => 0
 |b1::b' => bitToNat b1 + 2 * bitvecToNat b'
 end.
 
+(** For every bitvector there exists a number **)
 Lemma exists_number_bitvec:
 forall b:list bit, exists n:nat, bitvecToNat b = n.
 
@@ -66,21 +67,42 @@ intros. general induction b.
   + exists ((2*x)+1). simpl. rewrite H. omega. 
 Qed.
 
+(** Increment function which should be equal to the addition of 1 **)
 Fixpoint incr (b:bitvec) :=
 match b with
 | nil => I::nil
-| O::nil => I::nil
 | O::b' => I::b'
 | I::b' => O:: incr b'
 end .
 
-Compute (incr (incr nil)). 
+Lemma incr_eq_plus_one:
+forall (b:bitvec) (n:nat), bitvecToNat b = n -> bitvecToNat (incr b) = S n.
 
-(* min = a-(a-b)  *)
+Proof.
+intros. general induction b.
+- reflexivity.
+- assert (X: exists n', bitvecToNat (a::b) = n') by (exact (exists_number_bitvec (a::b))).
+  assert (X': exists n'', bitvecToNat b = n'') by (exact (exists_number_bitvec b)).
+  destruct X, X'. destruct a.
+  + reflexivity.
+  + simpl. rewrite (IHb x0 H0) in *. rewrite H0 in *. omega.
+Qed.
 
+Fixpoint decr (b:bitvec) :=
+match b with
+| nil => nil
+| O::nil => O::nil
+| I::b' => O::b'
+| O::b' => I::decr b'
+end.
+
+
+(** Define a min function for the recursion of the natToBitvec function. 
+It must be computed with min = a-(a-b)  **)
 Definition min a b :=
 a-(a-b).
 
+(** Define division by 2 as structural recursive function **)
 Fixpoint div2 n :=
 match n with
 |0 => 0
@@ -88,17 +110,23 @@ match n with
 |S (S n') => S(div2 (n'))
 end.
 
-(** TODO: Induction case of this proof. Maybe an additional Lemma is needed... *)
+(*
+(** TODO: Induction case of this proof. Maybe an additional Lemma is needed... **)
 Lemma always_smaller:
-forall n, min (S n) (S (div2 n)) = S (div2 n).
+forall n, min n (div2 n) = div2 n.
 
 Proof.
 intros.
 general induction n.
 - reflexivity.
-- simpl. admit. (* TODO!!! *)
+- simpl. destruct n.
+  + unfold min. omega.
+  +  unfold min. simpl. 
 Qed.
+*)
 
+(* TODO: Is a lemma needed that min always evaluates to div2 n? *)
+(** Define a function a function to compute the bitvector for a natural number **)
 Fixpoint natToBitvec (n:nat) :=
   match n with
     |0 => nil
@@ -110,6 +138,7 @@ Fixpoint natToBitvec (n:nat) :=
               end
 end.
 
+(** Forall natural numbers there exists a bitvector **)
 Lemma exists_bitvec_number:
 forall n:nat, exists b:bitvec, natToBitvec n = b.
 
@@ -121,21 +150,24 @@ intros. destruct n.
     * simpl. exists (I::nil). reflexivity.
     * simpl. exists (O::nil). reflexivity.
   + destruct (snd (divmod (S n) 1 0 0)).
-    * rewrite always_smaller. exists (I:: (natToBitvec (S (div2 n)))). reflexivity.
-    * rewrite always_smaller. exists (O:: (natToBitvec (S (div2 n)))). reflexivity.
+    * exists (I:: (natToBitvec (min (S n) (S (div2 n))))). reflexivity.
+    * exists (O:: (natToBitvec (min (S n) (S (div2 n))))). reflexivity.
 Qed.
 
+(*
 Lemma bijective_numbers:
-forall n:nat,
-bitvecToNat(natToBitvec n ) = n.
+forall (n:nat) (b:bitvec),
+natToBitvec n = b 
+<-> bitvecToNat b = n.
 
 Proof.
-intros. general induction n.
+intros.
 - reflexivity.
 - assert (X: exists b, natToBitvec (S n) = b) by (exact (exists_bitvec_number (S n))).
   destruct X. rewrite H.
   assert (Y: exists n, bitvecToNat x = n) by (exact (exists_number_bitvec (x))).
   destruct Y.
+*)
 
 Definition bitAnd (b1:bit) (b2:bit) :=
 match b1, b2 with
@@ -156,25 +188,6 @@ match b1, b2 with
 |_,_ => I
 end.
 
-Fixpoint bvAnd (a:bitvec) (b:bitvec) :=
-match a, b with
-|b1::a', b2::b' 
-  => (bitAnd b1 b2)::(bvAnd a' b')
-|_, nil
-  => a
-|_, _ => b
-end.
-
-Fixpoint bvOr (a:bitvec) (b:bitvec) :=
-match a,b with
-|b1::a',b2::b' 
-  => (bitOr b1 b2)::(bvOr a' b')
-|_, nil
-  => a
-|_,_ 
-  => b
-end.
-
 Fixpoint bvAdd (a:bitvec) (b:bitvec) (c:bit) :bitvec :=
 match a with
 |a1::a' =>  match b with
@@ -185,44 +198,96 @@ match a with
                |nil
                   => let r := bitXor a1 c in
                      let c':= bitAnd a1 c in
-                     r::(bvAdd a' nil c') 
+                       match c' with
+                           |O => r::a'
+                           |I => r::(incr a')
+                       end
                end
 |nil => match b with
             |b1::b'
                => let r := bitXor b1 c in
                   let c':= bitAnd b1 c in
-                      r::(bvAdd nil b' c' )
+                    match c' with
+                        | O => r:: b'
+                        | I => r::(incr b')
+                    end
             |nil
-               => c::nil
+               => match c with 
+                      | O => nil
+                      | I => I::nil
+                  end
        end
-end.
+end. 
 
 Lemma bit_bvAdd_lO:
 forall (v:bit) (b:bitvec), bvAdd (v::b) nil O = v::bvAdd b nil O.
 
 Proof.
-intros. simpl. unfold bitXor. destruct v; reflexivity.
+intros. simpl. unfold bitXor. unfold bitAnd. destruct v.
+- destruct b.
+  * simpl. reflexivity.
+  * simpl. unfold bitAnd. unfold bitXor. destruct b; reflexivity.
+- destruct b.
+  * reflexivity.
+  * simpl. unfold bitAnd. unfold bitXor. destruct b; reflexivity.
 Qed.
+
+Lemma bvAdd_nil_O:
+forall b, bvAdd b nil O = b.
+
+Proof.
+intros. general induction b.
+- reflexivity.
+- rewrite bit_bvAdd_lO. rewrite IHb. reflexivity.
+Qed.
+
 
 Lemma bit_bvAdd_lI:
 forall (v:bit) (b:bitvec), bvAdd (v::b) nil I = (bitXor v I)::bvAdd b nil v.
 
 Proof.
-intros. simpl. unfold bitXor. destruct v;  reflexivity.
+intros. simpl. unfold bitXor. destruct v.
+- simpl. rewrite bvAdd_nil_O. reflexivity.
+- unfold bitAnd. general induction b.
+  + reflexivity.
+  + simpl. unfold bitAnd. unfold bitXor. destruct a.
+    * reflexivity.
+    * reflexivity.
+Qed.
+
+Lemma bvAdd_nil_I:
+forall b, bvAdd b nil I = incr b.
+
+Proof.
+intros. general induction b.
+- reflexivity.
+- simpl. unfold bitAnd. unfold bitXor. destruct a; reflexivity.
 Qed.
 
 Lemma bit_bvAdd_rO:
 forall (v:bit) (b:bitvec), bvAdd nil (v::b) O = v:: bvAdd nil b O.
 
 Proof.
-intros. simpl. unfold bitXor. destruct v; reflexivity.
+intros. simpl. unfold bitAnd. unfold bitXor. destruct v. 
+- destruct b. 
+  + reflexivity.
+  + destruct b; reflexivity.
+- destruct b. 
+  + reflexivity.
+  + destruct b; reflexivity.
 Qed.
 
 Lemma bit_bvAdd_rI:
 forall (v:bit) (b:bitvec), bvAdd nil (v::b) I = (bitXor v I)::bvAdd nil b v.
 
 Proof.
-intros. simpl. unfold bitXor. destruct v; reflexivity.
+intros. simpl. unfold bitAnd. unfold bitXor. destruct v. 
+- destruct b. 
+  + reflexivity.
+  + destruct b; reflexivity.
+- destruct b.
+  + reflexivity.
+  + destruct b; reflexivity.
 Qed.
 
 Lemma bit_to_nat: 
@@ -232,6 +297,31 @@ Proof.
 intros. reflexivity.
 Qed.
 
+(* Definition bvAdd b1 b2 :=
+natToBitvec ((bitvecToNat b1) + (bitvecToNat b2)). 
+
+Lemma agree_on_add b1 b2 n1 n2:
+bitvecToNat b1 = n1
+-> bitvecToNat b2 = n2
+-> bvAdd b1 b2 O = natToBitvec(n1 + n2).
+
+Proof.
+intros. unfold bvAdd. rewrite H. rewrite H0. reflexivity.
+Qed.
+
+Definition bvSub b1 b2 :=
+natToBitvec ((bitvecToNat b1) - (bitvecToNat b2)).
+
+Lemma agree_on_sub b1 b2 n1 n2:
+bitvecToNat b1  = n1
+-> bitvecToNat b2 = n2
+-> bvSub b1 b2 = natToBitvec (n1-n2).
+
+Proof.
+intros. unfold bvSub. rewrite H. rewrite H0. reflexivity.
+Qed.
+*)
+
 Lemma agree_on_add b1 b2 n1 n2 c v:
 bitToNat c = v
 -> bitvecToNat b1 = n1 
@@ -240,13 +330,16 @@ bitToNat c = v
 
 Proof.
 general induction b1.
-- general induction b2.
-  + reflexivity.
-  + destruct a,c.
-    * rewrite (bit_bvAdd_rO O b2). erewrite bit_to_nat in *. rewrite IHb2. reflexivity.
-    * rewrite (bit_bvAdd_rI O b2). erewrite bit_to_nat in *. rewrite IHb2. unfold bitXor. reflexivity.
-    * rewrite (bit_bvAdd_rO I b2). erewrite bit_to_nat in *. rewrite IHb2. reflexivity.
-    * rewrite (bit_bvAdd_rI I b2). erewrite bit_to_nat in *. rewrite IHb2. unfold bitXor. simpl. omega.
+- destruct b2.
+  + destruct c. 
+    * reflexivity.
+    * reflexivity.
+  + destruct b,c.
+    * reflexivity.
+    * reflexivity.
+    * reflexivity.
+    * simpl. assert (A:exists n, bitvecToNat b2 = n) by (exact (exists_number_bitvec b2)).
+      destruct A. rewrite H in *.  rewrite (incr_eq_plus_one b2 H) in *. omega.
 - general induction b2.
   + destruct a,c.
     * rewrite (bit_bvAdd_lO O b1). rewrite (bit_to_nat O (bvAdd b1 nil O)). 
@@ -283,6 +376,7 @@ general induction b1.
     { rewrite H. rewrite H0. rewrite (IHb1 b2 x x0 I 1 H2 H H0). omega. }
     { rewrite H. rewrite H0. rewrite (IHb1 b2 x x0 I 1 H2 H H0). omega. }
 Qed.
+
 
 Fixpoint nGeqBool l r :bool :=
 match l, r with
@@ -323,6 +417,21 @@ match b with
 |a::b => false
 end.
 
+Lemma zero_decidable:
+forall b, decidable(isZero b).
+
+Proof.
+intros.
+destruct b.
+- unfold decidable. left. simpl. intuition.
+-  destruct b,b0.
+   + unfold decidable. left. simpl. intuition.
+   + unfold decidable. right. intuition.
+   + unfold decidable. right. intuition.
+   + unfold decidable. right. intuition.
+Qed.
+
+(*
 Lemma is_not_zero b:
 b <> nil /\ b <> O::nil -> isZero b = false.
 
@@ -335,6 +444,7 @@ intros. destruct b.
     * reflexivity. 
   + simpl. destruct b; reflexivity.
 Qed.
+*)
 
 Fixpoint bvMult' n (b:bitvec) akk :=
 match n with
@@ -350,6 +460,7 @@ end.
 Definition bvMult b1 b2 :=
 bvMult' (bitvecToNat b1) b2 b2.
 
+(*
 Lemma agree_on_mult b1 b2 n1 n2:
 bitvecToNat b1 = n1
 ->bitvecToNat b2 = n2
@@ -358,8 +469,8 @@ bitvecToNat b1 = n1
 Proof.
 intros. general induction b1.
 - reflexivity.
-- simpl. destruct n1, b2. 
-  + reflexivity. 
+- simpl.  destruct a. 
+  + simpl. unfold bvMult. 
   +  destruct b2.
   + simpl. unfold bvMult. destruct b1.
     * destruct a.
@@ -377,6 +488,8 @@ intros. general induction b1.
        { unfold bvMult. rewrite (is_not_zero H). 
          assert (H1: (O::b::b2) <> nil /\ (O::b::b2) <> O::nil) by (split; hnf; intros; discriminate).
          rewrite (is_not_zero H1). 
+*)
+
 Fixpoint nbvSub b c :=
 match b with 
   |a::b' => match  c,a with
@@ -387,6 +500,7 @@ match b with
             end
   |nil => nil
 end.
+
 
 Fixpoint bvSub (b1:bitvec) (b2:bitvec) (c:bit):=
 match bvGeq b1 b2 with
@@ -409,6 +523,21 @@ match bvGeq b1 b2 with
   |false => O::nil
 end.
 
+(** a / b = None, b = 0, Some ( S (a -b)/b) **)
+Fixpoint bvDiv' (a:nat) (b:bitvec) (akk:bitvec) :=
+match a with
+| 0 => Some akk
+| S n' => match b with
+           | nil => None
+           | O::nil => None
+           | _ => bvDiv' (min n' (a - (bitvecToNat b))) b (incr akk)
+          end
+end.
+
+Definition bvDiv (b1:bitvec) (b2:bitvec) :option bitvec:=
+bvDiv' (bitvecToNat b1) b2 (O::nil).
+
+(*
 Lemma nbvSub_decrease b c :
 bitvecToNat (nbvSub b c) = bitvecToNat b - bitToNat c.
 
@@ -466,6 +595,7 @@ intros. general induction b1.
     
   
   + admit.
+*)
 
 (**
 evalSexp evaluates an SMT expression given an environment with the variable bindings already 
@@ -475,6 +605,7 @@ a) a variable occurs free
 b) a variable has not been defined
 c) evaluation can become stuck
 **)
+
 Fixpoint evalSexp (E: senv)(s:sexp):option bitvec :=
 match s with
 |plus a b 
@@ -485,13 +616,32 @@ match s with
          | _, _ => None
      end
 |sub a b
-  => Some (nil)
+  => let v1 := evalSexp E a in
+     let v2 := evalSexp E b in
+     match v1,v2 with
+         | Some v1, Some v2 => Some (bvSub v1 v2 O)
+         | _,_=> None
+     end
 |mult a b
-  => Some (nil)
+  => let v1 := evalSexp E a in
+     let v2 := evalSexp E b in
+     match v1,v2 with
+         | Some v1, Some v2 => Some (bvMult v1 v2)
+         | _,_ => None
+     end
 |div a b  
-  => Some (nil)
-| neg a
-  => Some (nil)
+  => let v1 := evalSexp E a in
+     let v2 := evalSexp E b in
+     match v1, v2 with
+         | Some v1, Some v2 => bvDiv v1 v2
+         | _,_ => None
+     end
+| sneg v  (* TODO!*)
+ => let v' := evalSexp E v in
+    match v' with
+      | Some v => Some v 
+      | None => None
+    end
 | const c
   => Some c
 | svar v
