TransVal/smt.v
@@ -1,0 +1,170 @@
+Require Import List.
+Require Import IL Exp sexp.
+
+Set Implicit Arguments.
+
+(** Define what an argument list is **)
+Definition arglst := list sexp.
+
+(** Define what uninterpreted function symbols are **)
+Definition pred := lab (*arglst -> bool*).
+
+(** First define what an smt statement is **)
+Inductive smt :Type :=
+| smtAnd: smt -> smt -> smt
+| smtOr: smt -> smt -> smt
+| smtNeg: smt -> smt
+| ite: sexp -> smt -> smt -> smt
+| smtImp: smt -> smt -> smt
+| constr: sexp -> sexp -> smt
+| funcApp: pred -> arglst -> smt
+|smtReturn: sexp -> smt
+|smtFalse: smt.
+
+
+(** Now define the parameters for the translation function **)
+Inductive pol:Type :=
+| source :pol
+| target :pol.
+
+(** Helper function to merge SMT options **)
+Definition combine (o1:option smt) (o2:option smt) :option smt :=
+match o1, o2 with
+| Some v1, Some v2 => Some (smtAnd v1 v2)
+| Some v1, _ => o1
+| _, _  => o2
+end.
+
+(** Function to generate the guard expression for one expression **)
+Fixpoint undef (e:sexp) :=
+match e with
+|plus a b 
+ => combine (undef a) (undef b)
+|sub a b
+ => combine (undef a) (undef b)
+|mult a b
+ => combine (undef a) (undef b)
+|div a b
+ => let o1 := undef a in
+    let o2 := undef b in
+      match combine o1 o2 with
+          | Some v => Some (smtAnd v (smtNeg (constr b (const (O::nil)))))
+          | None => Some (smtNeg (constr b (const (O::nil))))
+    end
+| sneg a
+ => None
+|const c
+ => None
+|svar v
+ => None
+end. 
+
+(** Now the function that generates the guarding expressions for the smt translation function **)
+Fixpoint guard (p:pol) (e:sexp) (cont:smt) :=
+match p, undef e with
+|source, Some g
+ => smtAnd g cont
+|source, None
+ => cont
+|target, Some g
+ => smtImp g cont
+|target, None 
+ => cont
+end.
+
+Fixpoint guardList (p:pol) (l:arglst) (cont:smt) :=
+match l with
+| nil => cont
+| x:: l' => guardList p l' (guard p x cont)
+end.
+
+(** Define expression translation **)
+Fixpoint translateExp (e:exp) :option sexp :=
+match e with
+|Con v 
+ => Some ( const (natToBitvec(v)))
+|Var v
+ =>  Some (svar v)
+| UnOp op e
+ => match op, translateExp e with
+        | 0, Some v => Some (sneg v)
+        | _, _ =>  None
+    end
+|BinOp op e1 e2
+ =>  match translateExp e1, translateExp e2 with
+           | Some v1, Some v2 
+             => match op with
+                    | 0 => Some (plus v1 v2)
+                    | 1 => Some (sub v1 v2)
+                    | 2 => Some (mult v1 v2)
+                    | 3 => None (* TODO *)
+                    | 4 => None (* TODO *)
+                    | _ => None
+                end
+           |_, _ => None
+       end
+end.
+
+Fixpoint translateArgs (e:args) : option arglst :=
+match e with
+| nil => Some nil
+| x::e' 
+  => match translateExp x, translateArgs e'  with
+         | Some v, Some l => Some (v::l)
+         | _, _ => None
+     end
+end.
+
+Fixpoint translateStmt (s:stmt) (p:pol) :smt :=
+match s, p with
+(*let x = e in s' *)
+| stmtExp x e s', _ 
+  => let e' := translateExp e in
+        let x' := translateExp (Var x) in (* TODO: is this ok ? Hack from var to exp*)
+        let smt' := translateStmt s' p in
+        match x', e' with
+          | Some x' , Some v => guard  p  v   (smtAnd ( constr x' v) smt')
+          | _, _ => smtFalse
+        end
+(* if e then s else t *)
+| stmtIf e s t, _
+  => let s' := translateStmt s p in
+        let t' := translateStmt t p in
+        let e' := translateExp e in
+        match e' with
+            | Some v => guard  p  v ( ite v s' t')
+            | _ => smtFalse
+        end
+(* fun f x = t in s *)
+|  stmtLet x  t s, _ => smtFalse (* TODO *)
+(* extern ?? *)
+|  stmtExtern x f Y s, _ => smtFalse (* TODO *)
+(* f e, s*)
+| stmtGoto f e, source 
+  => match translateArgs e with
+         |Some l => guardList  source  l ( funcApp f l )
+         | None => smtFalse
+     end
+(* f e, t *)
+| stmtGoto f e, target  
+  => match translateArgs e with
+         | Some l => guardList target  l  ( smtNeg (funcApp f l ))
+         | None => smtFalse
+     end
+| stmtReturn e, source 
+  => match translateExp e with
+       |Some v => guard source  v  (smtReturn v)
+       | None => smtFalse
+     end
+| stmtReturn e, target 
+  => match translateExp e with
+         | Some v => guard  target  v ( smtNeg (smtReturn v))
+         | None => smtFalse
+     end
+end.
+
+(*
+*** Local Variables: ***
+*** coq-load-path: (("../" "Lvc")) ***
+*** End: ***
+*)
